library/init/data/nat/lemmas.lean
@@ -125,12 +125,12 @@ nat.le_trans (le_succ n) h
 protected lemma le_of_lt {n m : ℕ} (h : n < m) : n ≤ m :=
 le_of_succ_le h
 
-def lt.step {n m : ℕ} : n < m → n < succ m := less_than_or_equal.step
+lemma lt.step {n m : ℕ} : n < m → n < succ m := less_than_or_equal.step
 
-lemma eq_zero_or_pos (n : ℕ) : n = 0 ∨ n > 0 :=
+lemma eq_zero_or_pos (n : ℕ) : n = 0 ∨ 0 < n :=
 by {cases n, exact or.inl rfl, exact or.inr (succ_pos _)}
 
-protected lemma pos_of_ne_zero {n : nat} : n ≠ 0 → n > 0 :=
+protected lemma pos_of_ne_zero {n : nat} : n ≠ 0 → 0 < n :=
 or.resolve_left (eq_zero_or_pos n)
 
 protected lemma lt_trans {n m k : ℕ} (h₁ : n < m) : m < k → n < k :=
@@ -139,14 +139,14 @@ nat.le_trans (less_than_or_equal.step h₁)
 protected lemma lt_of_le_of_lt {n m k : ℕ} (h₁ : n ≤ m) : m < k → n < k :=
 nat.le_trans (succ_le_succ h₁)
 
-def lt.base (n : ℕ) : n < succ n := nat.le_refl (succ n)
+lemma lt.base (n : ℕ) : n < succ n := nat.le_refl (succ n)
 
 lemma lt_succ_self (n : ℕ) : n < succ n := lt.base n
 
 protected lemma le_antisymm {n m : ℕ} (h₁ : n ≤ m) : m ≤ n → n = m :=
 less_than_or_equal.cases_on h₁ (λ a, rfl) (λ a b c, absurd (nat.lt_of_le_of_lt b c) (nat.lt_irrefl n))
 
-protected lemma lt_or_ge : ∀ (a b : ℕ), a < b ∨ a ≥ b
+protected lemma lt_or_ge : ∀ (a b : ℕ), a < b ∨ b ≤ a
 | a 0     := or.inr (zero_le a)
 | a (b+1) :=
   match lt_or_ge a b with
@@ -260,10 +260,10 @@ lt_of_succ_le (add_succ k n ▸ nat.add_le_add_left (succ_le_of_lt h) k)
 protected lemma add_lt_add_right {n m : ℕ} (h : n < m) (k : ℕ) : n + k < m + k :=
 nat.add_comm k m ▸ nat.add_comm k n ▸ nat.add_lt_add_left h k
 
-protected lemma lt_add_of_pos_right {n k : ℕ} (h : k > 0) : n < n + k :=
+protected lemma lt_add_of_pos_right {n k : ℕ} (h : 0 < k) : n < n + k :=
 nat.add_lt_add_left h n
 
-protected lemma lt_add_of_pos_left {n k : ℕ} (h : k > 0) : n < k + n :=
+protected lemma lt_add_of_pos_left {n k : ℕ} (h : 0 < k) : n < k + n :=
 by rw nat.add_comm; exact nat.lt_add_of_pos_right h
 
 protected lemma add_lt_add {a b c d : ℕ} (h₁ : a < b) (h₂ : c < d) : a + c < b + d :=
@@ -285,13 +285,13 @@ end
 lemma mul_le_mul_right {n m : ℕ} (k : ℕ) (h : n ≤ m) : n * k ≤ m * k :=
 nat.mul_comm k m ▸ nat.mul_comm k n ▸ mul_le_mul_left k h
 
-protected lemma mul_lt_mul_of_pos_left {n m k : ℕ} (h : n < m) (hk : k > 0) : k * n < k * m :=
+protected lemma mul_lt_mul_of_pos_left {n m k : ℕ} (h : n < m) (hk : 0 < k) : k * n < k * m :=
 nat.lt_of_lt_of_le (nat.lt_add_of_pos_right hk) (mul_succ k n ▸ nat.mul_le_mul_left k (succ_le_of_lt h))
 
-protected lemma mul_lt_mul_of_pos_right {n m k : ℕ} (h : n < m) (hk : k > 0) : n * k < m * k :=
+protected lemma mul_lt_mul_of_pos_right {n m k : ℕ} (h : n < m) (hk : 0 < k) : n * k < m * k :=
 nat.mul_comm k m ▸ nat.mul_comm k n ▸ nat.mul_lt_mul_of_pos_left h hk
 
-protected lemma le_of_mul_le_mul_left {a b c : ℕ} (h : c * a ≤ c * b) (hc : c > 0) : a ≤ b :=
+protected lemma le_of_mul_le_mul_left {a b c : ℕ} (h : c * a ≤ c * b) (hc : 0 < c) : a ≤ b :=
 decidable.not_lt.1
   (assume h1 : b < a,
    have h2 : c * b < c * a, from nat.mul_lt_mul_of_pos_left h1 hc,
@@ -300,7 +300,7 @@ decidable.not_lt.1
 lemma le_of_lt_succ {m n : nat} : m < succ n → m ≤ n :=
 le_of_succ_le_succ
 
-theorem eq_of_mul_eq_mul_left {m k n : ℕ} (Hn : n > 0) (H : n * m = n * k) : m = k :=
+theorem eq_of_mul_eq_mul_left {m k n : ℕ} (Hn : 0 < n) (H : n * m = n * k) : m = k :=
 le_antisymm (nat.le_of_mul_le_mul_left (le_of_eq H) Hn)
             (nat.le_of_mul_le_mul_left (le_of_eq H.symm) Hn)
 
@@ -525,7 +525,7 @@ rfl
 theorem succ_sub_one (n : ℕ) : succ n - 1 = n :=
 rfl
 
-theorem succ_pred_eq_of_pos : ∀ {n : ℕ}, n > 0 → succ (pred n) = n
+theorem succ_pred_eq_of_pos : ∀ {n : ℕ}, 0 < n → succ (pred n) = n
 | 0 h        := absurd h (lt_irrefl 0)
 | (succ k) h := rfl
 
@@ -547,7 +547,7 @@ exists.elim (nat.le.dest h)
   (assume k, assume hk : n + k = m,
     by rw [← hk, nat.add_sub_cancel_left])
 
-protected theorem sub_add_cancel {n m : ℕ} (h : n ≥ m) : n - m + m = n :=
+protected theorem sub_add_cancel {n m : ℕ} (h : m ≤ n) : n - m + m = n :=
 by rw [nat.add_comm, add_sub_of_le h]
 
 protected theorem add_sub_assoc {m k : ℕ} (h : k ≤ m) (n : ℕ) : n + m - k = n + (m - k) :=
@@ -563,10 +563,10 @@ protected lemma lt_of_sub_eq_succ {m n l : ℕ} (H : m - n = nat.succ l) : n < m
 not_le.1
   (assume (H' : n ≥ m), begin simp [nat.sub_eq_zero_of_le H'] at H, contradiction end)
 
-@[simp] lemma zero_min (a : ℕ) : min 0 a = 0 :=
+lemma zero_min (a : ℕ) : min 0 a = 0 :=
 min_eq_left (zero_le a)
 
-@[simp] lemma min_zero (a : ℕ) : min a 0 = 0 :=
+lemma min_zero (a : ℕ) : min a 0 = 0 :=
 min_eq_right (zero_le a)
 
 -- Distribute succ over min
@@ -641,12 +641,12 @@ begin
   simp [if_neg, h]
 end
 
-lemma mod_eq_sub_mod {a b : nat} (h : a ≥ b) : a % b = (a - b) % b :=
+lemma mod_eq_sub_mod {a b : nat} (h : b ≤ a) : a % b = (a - b) % b :=
 or.elim (eq_zero_or_pos b)
   (λb0, by rw [b0, nat.sub_zero])
   (λh₂, by rw [mod_def, if_pos (and.intro h₂ h)])
 
-lemma mod_lt (x : nat) {y : nat} (h : y > 0) : x % y < y :=
+lemma mod_lt (x : nat) {y : nat} (h : 0 < y) : x % y < y :=
 begin
   induction x using nat.case_strong_induction_on with x ih,
   { rw zero_mod, assumption },
@@ -723,7 +723,7 @@ protected lemma div_le_self : ∀ (m n : ℕ), m / n ≤ m
    ... ≤ succ n * m : mul_le_mul_right _ (succ_le_succ (zero_le _)),
   nat.div_le_of_le_mul this
 
-lemma div_eq_sub_div {a b : nat} (h₁ : b > 0) (h₂ : a ≥ b) : a / b = (a - b) / b + 1 :=
+lemma div_eq_sub_div {a b : nat} (h₁ : 0 < b) (h₂ : b ≤ a) : a / b = (a - b) / b + 1 :=
 begin
   rw [div_def a, if_pos],
   split ; assumption
@@ -741,9 +741,7 @@ end
 -- with
 --   f x = x * k
 --   g y = y / k
-theorem le_div_iff_mul_le (x y : ℕ) {k : ℕ}
-  (Hk : k > 0)
-: x ≤ y / k ↔ x * k ≤ y :=
+theorem le_div_iff_mul_le (x y : ℕ) {k : ℕ} (Hk : 0 < k) : x ≤ y / k ↔ x * k ≤ y :=
 begin
   -- Hk is needed because, despite div being made total, y / 0 := 0
   --     x * 0 ≤ y ↔ x ≤ y / 0
@@ -776,9 +774,7 @@ begin
      } }
 end
 
-theorem div_lt_iff_lt_mul (x y : ℕ) {k : ℕ}
-  (Hk : k > 0)
-: x / k < y ↔ x < y * k :=
+theorem div_lt_iff_lt_mul (x y : ℕ) {k : ℕ} (Hk : 0 < k) : x / k < y ↔ x < y * k :=
 begin
   simp [← not_le],
   apply not_iff_not_of_iff,
@@ -801,18 +797,18 @@ by cases n; simp
 theorem exists_eq_succ_of_ne_zero {n : ℕ} (H : n ≠ 0) : ∃k : ℕ, n = succ k :=
 ⟨_, (eq_zero_or_eq_succ_pred _).resolve_left H⟩
 
-theorem discriminate {B : Sort u} {n : ℕ} (H1: n = 0 → B) (H2 : ∀m, n = succ m → B) : B :=
+def discriminate {B : Sort u} {n : ℕ} (H1: n = 0 → B) (H2 : ∀m, n = succ m → B) : B :=
 by induction h : n; [exact H1 h, exact H2 _ h]
 
 theorem one_succ_zero : 1 = succ 0 := rfl
 
-theorem two_step_induction {P : ℕ → Sort u} (H1 : P 0) (H2 : P 1)
+def two_step_induction {P : ℕ → Sort u} (H1 : P 0) (H2 : P 1)
     (H3 : ∀ (n : ℕ) (IH1 : P n) (IH2 : P (succ n)), P (succ (succ n))) : Π (a : ℕ), P a
 | 0               := H1
 | 1               := H2
 | (succ (succ n)) := H3 _ (two_step_induction _) (two_step_induction _)
 
-theorem sub_induction {P : ℕ → ℕ → Sort u} (H1 : ∀m, P 0 m)
+def sub_induction {P : ℕ → ℕ → Sort u} (H1 : ∀m, P 0 m)
    (H2 : ∀n, P (succ n) 0) (H3 : ∀n m, P n m → P (succ n) (succ m)) : Π (n m : ℕ), P n m
 | 0        m        := H1 _
 | (succ n) 0        := H2 _
@@ -853,7 +849,7 @@ le_lt_antisymm h₂ h₁
 protected theorem lt_asymm {n m : ℕ} (h₁ : n < m) : ¬ m < n :=
 le_lt_antisymm (nat.le_of_lt h₁)
 
-protected def lt_ge_by_cases {a b : ℕ} {C : Sort u} (h₁ : a < b → C) (h₂ : a ≥ b → C) : C :=
+protected def lt_ge_by_cases {a b : ℕ} {C : Sort u} (h₁ : a < b → C) (h₂ : b ≤ a → C) : C :=
 decidable.by_cases h₁ (λ h, h₂ (or.elim (nat.lt_or_ge a b) (λ a, absurd a h) (λ a, a)))
 
 protected def lt_by_cases {a b : ℕ} {C : Sort u} (h₁ : a < b → C) (h₂ : a = b → C)
@@ -869,7 +865,7 @@ protected theorem eq_or_lt_of_not_lt {a b : ℕ} (hnlt : ¬ a < b) : a = b ∨ b
 
 theorem lt_succ_of_lt {a b : nat} (h : a < b) : a < succ b := le_succ_of_le h
 
-def one_pos := nat.zero_lt_one
+lemma one_pos : 0 < 1 := nat.zero_lt_one
 
 /- subtraction -/
 
@@ -906,12 +902,12 @@ begin
   simp [nat.right_distrib, nat.left_distrib, nat.add_left_comm, nat.mul_one, nat.one_mul, nat.add_assoc],
 end
 
-theorem succ_sub {m n : ℕ} (h : m ≥ n) : succ m - n = succ (m - n) :=
+theorem succ_sub {m n : ℕ} (h : n ≤ m) : succ m - n = succ (m - n) :=
 exists.elim (nat.le.dest h)
   (assume k, assume hk : n + k = m,
     by rw [← hk, nat.add_sub_cancel_left, ← add_succ, nat.add_sub_cancel_left])
 
-protected theorem sub_pos_of_lt {m n : ℕ} (h : m < n) : n - m > 0 :=
+protected theorem sub_pos_of_lt {m n : ℕ} (h : m < n) : 0 < n - m :=
 have 0 + m < n - m + m, begin rw [nat.zero_add, nat.sub_add_cancel (le_of_lt h)], exact h end,
 nat.lt_of_add_lt_add_right this
 
@@ -930,7 +926,7 @@ theorem sub_one_sub_lt {n i} (h : i < n) : n - 1 - i < n := begin
   apply nat.zero_lt_succ
 end
 
-theorem pred_inj : ∀ {a b : nat}, a > 0 → b > 0 → nat.pred a = nat.pred b → a = b
+theorem pred_inj : ∀ {a b : nat}, 0 < a → 0 < b → nat.pred a = nat.pred b → a = b
 | (succ a) (succ b) ha hb h := have a = b, from h, by rw this
 | (succ a) 0        ha hb h := absurd hb (lt_irrefl _)
 | 0        (succ b) ha hb h := absurd ha (lt_irrefl _)
@@ -1065,49 +1061,49 @@ theorem div_mul_le_self : ∀ (m n : ℕ), m / n * n ≤ m
 | m 0        := by simp; apply zero_le
 | m (succ n) := (le_div_iff_mul_le _ _ (nat.succ_pos _)).1 (le_refl _)
 
-@[simp] theorem add_div_right (x : ℕ) {z : ℕ} (H : z > 0) : (x + z) / z = succ (x / z) :=
+@[simp] theorem add_div_right (x : ℕ) {z : ℕ} (H : 0 < z) : (x + z) / z = succ (x / z) :=
 by rw [div_eq_sub_div H (nat.le_add_left _ _), nat.add_sub_cancel]
 
-@[simp] theorem add_div_left (x : ℕ) {z : ℕ} (H : z > 0) : (z + x) / z = succ (x / z) :=
+@[simp] theorem add_div_left (x : ℕ) {z : ℕ} (H : 0 < z) : (z + x) / z = succ (x / z) :=
 by rw [nat.add_comm, add_div_right x H]
 
-@[simp] theorem mul_div_right (n : ℕ) {m : ℕ} (H : m > 0) : m * n / m = n :=
+@[simp] theorem mul_div_right (n : ℕ) {m : ℕ} (H : 0 < m) : m * n / m = n :=
 by {induction n; simp [*, mul_succ, nat.mul_zero] }
 
-@[simp] theorem mul_div_left (m : ℕ) {n : ℕ} (H : n > 0) : m * n / n = m :=
+@[simp] theorem mul_div_left (m : ℕ) {n : ℕ} (H : 0 < n) : m * n / n = m :=
 by rw [nat.mul_comm, mul_div_right _ H]
 
-protected theorem div_self {n : ℕ} (H : n > 0) : n / n = 1 :=
+protected theorem div_self {n : ℕ} (H : 0 < n) : n / n = 1 :=
 let t := add_div_right 0 H in by rwa [nat.zero_add, nat.zero_div] at t
 
-theorem add_mul_div_left (x z : ℕ) {y : ℕ} (H : y > 0) : (x + y * z) / y = x / y + z :=
+theorem add_mul_div_left (x z : ℕ) {y : ℕ} (H : 0 < y) : (x + y * z) / y = x / y + z :=
 begin
   induction z with z ih,
   { rw [nat.mul_zero, nat.add_zero, nat.add_zero] },
   { rw [mul_succ, ← nat.add_assoc, add_div_right _ H, ih] }
 end
 
-theorem add_mul_div_right (x y : ℕ) {z : ℕ} (H : z > 0) : (x + y * z) / z = x / z + y :=
+theorem add_mul_div_right (x y : ℕ) {z : ℕ} (H : 0 < z) : (x + y * z) / z = x / z + y :=
 by rw [nat.mul_comm, add_mul_div_left _ _ H]
 
-protected theorem mul_div_cancel (m : ℕ) {n : ℕ} (H : n > 0) : m * n / n = m :=
+protected theorem mul_div_cancel (m : ℕ) {n : ℕ} (H : 0 < n) : m * n / n = m :=
 let t := add_mul_div_right 0 m H in by rwa [nat.zero_add, nat.zero_div, nat.zero_add] at t
 
-protected theorem mul_div_cancel_left (m : ℕ) {n : ℕ} (H : n > 0) : n * m / n = m :=
+protected theorem mul_div_cancel_left (m : ℕ) {n : ℕ} (H : 0 < n) : n * m / n = m :=
 by rw [nat.mul_comm, nat.mul_div_cancel _ H]
 
-protected theorem div_eq_of_eq_mul_left {m n k : ℕ} (H1 : n > 0) (H2 : m = k * n) :
+protected theorem div_eq_of_eq_mul_left {m n k : ℕ} (H1 : 0 < n) (H2 : m = k * n) :
   m / n = k :=
 by rw [H2, nat.mul_div_cancel _ H1]
 
-protected theorem div_eq_of_eq_mul_right {m n k : ℕ} (H1 : n > 0) (H2 : m = n * k) :
+protected theorem div_eq_of_eq_mul_right {m n k : ℕ} (H1 : 0 < n) (H2 : m = n * k) :
   m / n = k :=
 by rw [H2, nat.mul_div_cancel_left _ H1]
 
 protected theorem div_eq_of_lt_le {m n k : ℕ}
   (lo : k * n ≤ m) (hi : m < succ k * n) :
   m / n = k :=
-have npos : n > 0, from (eq_zero_or_pos _).resolve_left $ λ hn,
+have npos : 0 < n, from (eq_zero_or_pos _).resolve_left $ λ hn,
   by rw [hn, nat.mul_zero] at hi lo; exact absurd lo (not_le_of_gt hi),
 le_antisymm
   (le_of_lt_succ ((nat.div_lt_iff_lt_mul _ _ npos).2 hi))
@@ -1115,7 +1111,7 @@ le_antisymm
 
 theorem mul_sub_div (x n p : ℕ) (h₁ : x < n*p) : (n * p - succ x) / n = p - succ (x / n) :=
 begin
-  have npos : n > 0 := (eq_zero_or_pos _).resolve_left (λ n0,
+  have npos : 0 < n := (eq_zero_or_pos _).resolve_left (λ n0,
     by rw [n0, nat.zero_mul] at h₁; exact not_lt_zero _ h₁),
   apply nat.div_eq_of_lt_le,
   { rw [nat.mul_sub_right_distrib, nat.mul_comm],
@@ -1129,7 +1125,7 @@ begin
     { apply (div_lt_iff_lt_mul _ _ npos).2, rwa nat.mul_comm } }
 end
 
-protected lemma mul_pos {a b : ℕ} (ha : a > 0) (hb : b > 0) : a * b > 0 :=
+protected lemma mul_pos {a b : ℕ} (ha : 0 < a) (hb : 0 < b) : 0 < a * b :=
 have h : 0 * b < a * b, from nat.mul_lt_mul_of_pos_right ha hb,
 by rwa nat.zero_mul at h
 
@@ -1150,12 +1146,11 @@ begin
     refl }
 end
 
-protected theorem mul_div_mul {m : ℕ} (n k : ℕ) (H : m > 0) : m * n / (m * k) = n / k :=
+protected theorem mul_div_mul {m : ℕ} (n k : ℕ) (H : 0 < m) : m * n / (m * k) = n / k :=
 by rw [← nat.div_div_eq_div_mul, nat.mul_div_cancel_left _ H]
 
 /- dvd -/
 
-@[simp]
 protected theorem dvd_mul_right (a b : ℕ) : a ∣ a * b := ⟨b, rfl⟩
 
 protected theorem dvd_trans {a b c : ℕ} (h₁ : a ∣ b) (h₂ : b ∣ c) : a ∣ c :=
@@ -1186,7 +1181,7 @@ theorem dvd_mod_iff {k m n : ℕ} (h : k ∣ n) : k ∣ m % n ↔ k ∣ m :=
 let t := @nat.dvd_add_iff_left _ (m % n) _ (nat.dvd_trans h (nat.dvd_mul_right n (m / n))) in
 by rwa mod_add_div at t
 
-theorem le_of_dvd {m n : ℕ} (h : n > 0) : m ∣ n → m ≤ n :=
+theorem le_of_dvd {m n : ℕ} (h : 0 < n) : m ∣ n → m ≤ n :=
 λ⟨k, e⟩, by {
   revert h, rw e, refine k.cases_on _ _,
   exact λhn, absurd hn (lt_irrefl _),
@@ -1197,7 +1192,7 @@ theorem dvd_antisymm : Π {m n : ℕ}, m ∣ n → n ∣ m → m = n
 | 0        n        h₁ h₂ := (nat.eq_zero_of_zero_dvd h₁).symm
 | (succ m) (succ n) h₁ h₂ := le_antisymm (le_of_dvd (succ_pos _) h₁) (le_of_dvd (succ_pos _) h₂)
 
-theorem pos_of_dvd_of_pos {m n : ℕ} (H1 : m ∣ n) (H2 : n > 0) : m > 0 :=
+theorem pos_of_dvd_of_pos {m n : ℕ} (H1 : m ∣ n) (H2 : 0 < n) : 0 < m :=
 nat.pos_of_ne_zero $ λm0, by rw m0 at H1; rw nat.eq_zero_of_zero_dvd H1 at H2; exact lt_irrefl _ H2
 
 theorem eq_one_of_dvd_one {n : ℕ} (H : n ∣ 1) : n = 1 :=
@@ -1227,10 +1222,10 @@ or.elim (eq_zero_or_pos k)
   (λh, have m * n / k = m * (n / k * k) / k, by rw nat.div_mul_cancel H,
        by rw[this, ← nat.mul_assoc, nat.mul_div_cancel _ h])
 
-theorem dvd_of_mul_dvd_mul_left {m n k : ℕ} (kpos : k > 0) (H : k * m ∣ k * n) : m ∣ n :=
+theorem dvd_of_mul_dvd_mul_left {m n k : ℕ} (kpos : 0 < k) (H : k * m ∣ k * n) : m ∣ n :=
 exists.elim H (λl H1, by rw nat.mul_assoc at H1; exact ⟨_, eq_of_mul_eq_mul_left kpos H1⟩)
 
-theorem dvd_of_mul_dvd_mul_right {m n k : ℕ} (kpos : k > 0) (H : m * k ∣ n * k) : m ∣ n :=
+theorem dvd_of_mul_dvd_mul_right {m n k : ℕ} (kpos : 0 < k) (H : m * k ∣ n * k) : m ∣ n :=
 by rw [nat.mul_comm m k, nat.mul_comm n k] at H; exact dvd_of_mul_dvd_mul_left kpos H
 
 /- --- -/
@@ -1266,10 +1261,10 @@ calc
   a * b ≤ c * b : nat.mul_le_mul_of_nonneg_right hac
     ... ≤ c * d : nat.mul_le_mul_of_nonneg_left hbd
 
-lemma div_lt_self {n m : nat} : n > 0 → m > 1 → n / m < n :=
+lemma div_lt_self {n m : nat} : 0 < n → 1 < m → n / m < n :=
 begin
   intros h₁ h₂,
-  have m_pos : m > 0, { apply lt_trans _ h₂, comp_val },
+  have m_pos : 0 < m, { apply lt_trans _ h₂, comp_val },
   suffices : 1 * n < m * n, {
     rw [nat.one_mul, nat.mul_comm] at this,
     exact iff.mpr (nat.div_lt_iff_lt_mul n n m_pos) this
