library/init/data/int/basic.lean
@@ -213,7 +213,7 @@ sub_nat_nat_elim m n (λm n i, sub_nat_nat (m + k) (n + k) = i)
   (assume i m, have m + i + 1 + k = (m + k) + i + 1, by simp [nat.add_comm, nat.add_left_comm],
     begin rw [this], exact sub_nat_nat_add_right end)
 
-lemma sub_nat_nat_of_ge {m n : ℕ} (h : m ≥ n) : sub_nat_nat m n = of_nat (m - n) :=
+lemma sub_nat_nat_of_le {m n : ℕ} (h : n ≤ m) : sub_nat_nat m n = of_nat (m - n) :=
 sub_nat_nat_of_sub_eq_zero (sub_eq_zero_of_le h)
 
 lemma sub_nat_nat_of_lt {m n : ℕ} (h : m < n) : sub_nat_nat m n = -[1+ pred (n - m)] :=
@@ -232,7 +232,7 @@ lemma eq_zero_of_nat_abs_eq_zero : Π {a : ℤ}, nat_abs a = 0 → a = 0
 | (of_nat m) H := congr_arg of_nat H
 | -[1+ m']   H := absurd H (succ_ne_zero _)
 
-lemma nat_abs_pos_of_ne_zero {a : ℤ} (h : a ≠ 0) : nat_abs a > 0 :=
+lemma nat_abs_pos_of_ne_zero {a : ℤ} (h : a ≠ 0) : 0 < nat_abs a :=
 (eq_zero_or_pos _).resolve_left $ mt eq_zero_of_nat_abs_eq_zero h
 
 lemma nat_abs_zero : nat_abs (0 : int) = (0 : nat) := rfl
@@ -337,7 +337,7 @@ protected lemma add_zero : ∀ a : ℤ, a + 0 = a
 protected lemma zero_add (a : ℤ) : 0 + a = a :=
 int.add_comm a 0 ▸ int.add_zero a
 
-lemma sub_nat_nat_sub {m n : ℕ} (h : m ≥ n) (k : ℕ) :
+lemma sub_nat_nat_sub {m n : ℕ} (h : n ≤ m) (k : ℕ) :
   sub_nat_nat (m - n) k = sub_nat_nat m (k + n) :=
 calc
   sub_nat_nat (m - n) k = sub_nat_nat (m - n + n) (k + n) : by rewrite [sub_nat_nat_add_add]
@@ -347,9 +347,9 @@ lemma sub_nat_nat_add (m n k : ℕ) : sub_nat_nat (m + n) k = of_nat m + sub_nat
 begin
   have h := decidable.le_or_lt k n,
   cases h with h' h',
-  { rw [sub_nat_nat_of_ge h'],
+  { rw [sub_nat_nat_of_le h'],
     have h₂ : k ≤ m + n, exact (le_trans h' (le_add_left _ _)),
-    rw [sub_nat_nat_of_ge h₂], simp,
+    rw [sub_nat_nat_of_le h₂], simp,
     rw nat.add_sub_assoc h' },
   rw [sub_nat_nat_of_lt h'], simp, rw [succ_pred_eq_of_pos (nat.sub_pos_of_lt h')],
   transitivity, rw [← nat.sub_add_cancel (le_of_lt h')],
@@ -361,7 +361,7 @@ lemma sub_nat_nat_add_neg_succ_of_nat (m n k : ℕ) :
 begin
   have h := decidable.le_or_lt n m,
   cases h with h' h',
-  { rw [sub_nat_nat_of_ge h'], simp, rw [sub_nat_nat_sub h', nat.add_comm] },
+  { rw [sub_nat_nat_of_le h'], simp, rw [sub_nat_nat_sub h', nat.add_comm] },
   have h₂ : m < n + succ k, exact nat.lt_of_lt_of_le h' (le_add_right _ _),
   have h₃ : m ≤ n + k, exact le_of_succ_le_succ h₂,
   rw [sub_nat_nat_of_lt h', sub_nat_nat_of_lt h₂], simp [nat.add_comm],
@@ -476,7 +476,7 @@ begin
       rw [← succ_pred_eq_of_pos (nat.sub_pos_of_lt h')], reflexivity },
     have h' : m * k ≤ m * n,
       exact mul_le_mul_left _ h,
-    rw [sub_nat_nat_of_ge h, sub_nat_nat_of_ge h'], simp,
+    rw [sub_nat_nat_of_le h, sub_nat_nat_of_le h'], simp,
     rw [nat.mul_sub_left_distrib]
   },
   have h₂ : of_nat 0 = 0, exact rfl,
@@ -502,14 +502,14 @@ begin
   cases h with h h,
   { have h' : succ m * n < succ m * k,
       exact nat.mul_lt_mul_of_pos_left h (nat.succ_pos m),
-    rw [sub_nat_nat_of_lt h, sub_nat_nat_of_ge (le_of_lt h')],
+    rw [sub_nat_nat_of_lt h, sub_nat_nat_of_le (le_of_lt h')],
     simp [succ_pred_eq_of_pos (nat.sub_pos_of_lt h), nat.mul_sub_left_distrib]},
   have h' : n > k ∨ k = n,
     exact decidable.lt_or_eq_of_le h,
   cases h' with h' h',
   { have h₁ : succ m * n > succ m * k,
       exact nat.mul_lt_mul_of_pos_left h' (nat.succ_pos m),
-    rw [sub_nat_nat_of_ge h, sub_nat_nat_of_lt h₁], simp [nat.mul_sub_left_distrib, nat.mul_comm],
+    rw [sub_nat_nat_of_le h, sub_nat_nat_of_lt h₁], simp [nat.mul_sub_left_distrib, nat.mul_comm],
     rw [nat.mul_comm k, nat.mul_comm n, ← succ_pred_eq_of_pos (nat.sub_pos_of_lt h₁),
         ← neg_of_nat_of_succ],
     reflexivity },
